src/Examples/StatDb/WeakestPre.v
@@ -17,7 +17,7 @@ Definition reg_map `{statG Σ} (i: Var.id) (v: nat) :=
   own (stat_reg_gnames i) (◯ (Excl' v)).
 Definition reg_map_auth `{statG Σ} (i: Var.id) (v: nat) :=
   own (stat_reg_gnames i) (● (Excl' v)).
-  
+
 Local Notation "i ↦ v" := (reg_map i v) (at level 20) : bi_scope.
 Local Notation "i ↦● v" := (reg_map_auth i v) (at level 20) : bi_scope.
 
@@ -29,7 +29,7 @@ Instance statG_irisG `{statG Σ} : irisG Var.Op Var.l Σ :=
     iris_invG := stat_invG;
     state_interp := (λ '(ns, nc, nl), Var.Sum ↦● ns ∗ Var.Count ↦● nc ∗ Var.Lock ↦● nl)%I
   }.
-                                     
+
 
 Section lifting.
 Context `{statG Σ}.
@@ -42,27 +42,85 @@ Proof.
     done.
 Qed.
 
+Lemma reg_agree i v1 v2 : i ↦ v1 -∗ i ↦● v2 -∗ ⌜ v1 = v2 ⌝.
+Proof.
+  iIntros "Hf Ha".
+    by iDestruct (own_valid_2 with "Ha Hf")
+      as %[<-%Excl_included%leibniz_equiv _]%auth_valid_discrete_2.
+Qed.
+
+Ltac destruct_state σ H :=
+  destruct σ as ((?&?)&?);
+  iDestruct H as "(?&?&?)".
+
 Lemma wp_write s E i v' v :
   {{{ ▷ i ↦ v' }}} write i v @ s; E {{{ RET tt; i ↦ v }}}.
 Proof.
-  iIntros (Φ) ">Hi HΦ".
-  iApply wp_lift_atomic_step; first done.
-  iIntros (σ) "Hown". destruct σ as ((ns&nc)&nl).
-  iDestruct "Hown" as "(Howns&Hownc&Hownl)".
-  iModIntro. iSplit.
-  {
-    destruct s; auto. iPureIntro. rewrite /non_errorable => Hin.
-    apply bind_pure_no_err in Hin.
-    inversion Hin.
-  }
-  iIntros (e2 σ2 efs Hstep).
-  iNext.
-  destruct Hstep as ([]&?&Hstep&Hpure).
+  iIntros (Φ) ">Hi HΦ". iApply wp_lift_call_step.
+  iIntros (σ) "Hown". destruct_state σ "Hown".
+  iModIntro. iSplit; first by destruct s.
+  iIntros (e2 σ2 Hstep) "!>".
   inversion Hstep; subst.
-  inversion Hpure; subst.
-  destruct i; simpl; iFrame;
+  destruct i; iFrame;
   iMod (reg_update _ v with "Hi [$]") as "(Hi&$)";
-  iSplitR ""; auto;
-  iModIntro; by iApply "HΦ".
+  by iApply "HΦ".
 Qed.
+
+Lemma wp_read s E i v :
+  {{{ ▷ i ↦ v }}} read i @ s; E {{{ RET v; i ↦ v }}}.
+Proof.
+  iIntros (Φ) ">Hi HΦ". iApply wp_lift_call_step.
+  iIntros (σ) "Hown". destruct_state σ "Hown".
+  iModIntro. iSplit; first by destruct s.
+  iIntros (e2 σ2 Hstep) "!>".
+  inversion Hstep; subst.
+  destruct i; iDestruct (reg_agree with "Hi [$]") as "%"; subst;
+    iFrame; simpl; by iApply "HΦ".
+Qed.
+
+Lemma cas_non_stuck i v1 v2 σ:
+  ¬ Var.l.(step) (CAS i v1 v2) σ Err.
+Proof.
+  intros Hstuck. destruct Hstuck as [Hread|(v'&?&Hread&Hrest)].
+  - inversion Hread.
+  - destruct nat_eq_dec; subst; [apply bind_pure_no_err in Hrest|]; inversion Hrest.
+Qed.
+
+Lemma wp_cas_fail s E i v1 v2 v3 :
+  v1 ≠ v2 →
+  {{{ ▷ i ↦ v1 }}} cas i v2 v3 @ s; E {{{ RET v1; i ↦ v1 }}}.
+Proof.
+  iIntros (Hneq Φ) ">Hi HΦ". iApply wp_lift_call_step.
+  iIntros (σ) "Hown". destruct_state σ "Hown".
+  iModIntro. iSplit.
+  { destruct s; auto using cas_non_stuck. }
+  iIntros (e2 σ2 Hstep) "!>".
+  inversion Hstep as (v'&σ2'&Hread&Hrest); subst.
+  inversion Hread; subst.
+  destruct i; iDestruct (reg_agree with "Hi [$]") as "%"; subst;
+    iFrame; simpl;
+  (destruct (nat_eq_dec); [ by (subst; exfalso; eauto)|];
+  inversion Hrest; subst;
+  iFrame; by iApply "HΦ").
+Qed.
+
+Lemma wp_cas_suc s E i v1 v2 :
+  {{{ ▷ i ↦ v1 }}} cas i v1 v2 @ s; E {{{ RET v1; i ↦ v2 }}}.
+Proof.
+  iIntros (Φ) ">Hi HΦ". iApply wp_lift_call_step.
+  iIntros (σ) "Hown". destruct_state σ "Hown".
+  iModIntro. iSplit.
+  { destruct s; auto using cas_non_stuck. }
+  iIntros (e2 σ2 Hstep) "!>".
+  inversion Hstep as (v'&σ2'&Hread&Hrest); subst.
+  inversion Hread; subst.
+  destruct i; iDestruct (reg_agree with "Hi [$]") as "%"; subst;
+  (destruct (nat_eq_dec); [| simpl in *; congruence]);
+  inversion Hrest as ([]&?&Hputs&Hpure); inversion Hputs; inversion Hpure; subst;
+     iMod (reg_update _ v2 with "Hi [$]") as "(Hi&$)"; subst;
+    iFrame; simpl;
+  inversion Hrest; subst;
+  iFrame; by iApply "HΦ".
+Qed.
+
 End lifting.
